Zcash/Circuits/Integration/TopLevelInterpretation.lean
@@ -2,11 +2,10 @@ import Zcash.Circuits.Integration.FixedColumns
 import Zcash.Circuits.Halo2.ConstraintsCompiled
 import Zcash.Common.RelationWitness
 import Zcash.Snark.Soundness.Multiopen.InstanceColumns
-import Zcash.Circuits.Integration.TopLevelLookups
+import Zcash.Circuits.Integration.PolynomialConstraints
 import Zcash.Snark.Soundness.Multiopen.CanonicalRelation
-import Zcash.Circuits.Integration.TopLevelGates
-import Zcash.Circuits.Integration.TopLevelWitness
-import Zcash.Circuits.Integration.TopLevelCopyConstraints
+import Zcash.Circuits.Integration.Assignment
+import Zcash.Circuits.Integration.Permutation
 import Zcash.Snark.Keygen.Pipeline
 import Mathlib.Util.AssertNoSorry
 
